proofs/fstar/extraction/Libcrux.Kem.Kyber.Types.fst
@@ -153,7 +153,7 @@ let impl_18__split_at (v_SIZE: usize) (self: t_KyberPublicKey v_SIZE) (mid: usiz
     : (t_Slice u8 & t_Slice u8) =
   Core.Slice.impl__split_at (Rust_primitives.unsize self.f_value <: t_Slice u8) mid
 
-type t_KyberKeyPair (v_PRIVATE_KEY_SIZE: usize) (v_PUBLIC_KEY_SIZE: usize) = {
+type t_MlKemKeyPair (v_PRIVATE_KEY_SIZE: usize) (v_PUBLIC_KEY_SIZE: usize) = {
   f_sk:t_KyberPrivateKey v_PRIVATE_KEY_SIZE;
   f_pk:t_KyberPublicKey v_PUBLIC_KEY_SIZE
 }
@@ -162,34 +162,34 @@ let impl__from
       (v_PRIVATE_KEY_SIZE v_PUBLIC_KEY_SIZE: usize)
       (sk: t_KyberPrivateKey v_PRIVATE_KEY_SIZE)
       (pk: t_KyberPublicKey v_PUBLIC_KEY_SIZE)
-    : t_KyberKeyPair v_PRIVATE_KEY_SIZE v_PUBLIC_KEY_SIZE =
-  { f_sk = sk; f_pk = pk } <: t_KyberKeyPair v_PRIVATE_KEY_SIZE v_PUBLIC_KEY_SIZE
+    : t_MlKemKeyPair v_PRIVATE_KEY_SIZE v_PUBLIC_KEY_SIZE =
+  { f_sk = sk; f_pk = pk } <: t_MlKemKeyPair v_PRIVATE_KEY_SIZE v_PUBLIC_KEY_SIZE
 
 let impl__new
       (v_PRIVATE_KEY_SIZE v_PUBLIC_KEY_SIZE: usize)
       (sk: t_Array u8 v_PRIVATE_KEY_SIZE)
       (pk: t_Array u8 v_PUBLIC_KEY_SIZE)
-    : t_KyberKeyPair v_PRIVATE_KEY_SIZE v_PUBLIC_KEY_SIZE =
+    : t_MlKemKeyPair v_PRIVATE_KEY_SIZE v_PUBLIC_KEY_SIZE =
   { f_sk = Core.Convert.f_into sk; f_pk = Core.Convert.f_into pk }
   <:
-  t_KyberKeyPair v_PRIVATE_KEY_SIZE v_PUBLIC_KEY_SIZE
+  t_MlKemKeyPair v_PRIVATE_KEY_SIZE v_PUBLIC_KEY_SIZE
 
 let impl__pk
       (v_PRIVATE_KEY_SIZE v_PUBLIC_KEY_SIZE: usize)
-      (self: t_KyberKeyPair v_PRIVATE_KEY_SIZE v_PUBLIC_KEY_SIZE)
+      (self: t_MlKemKeyPair v_PRIVATE_KEY_SIZE v_PUBLIC_KEY_SIZE)
     : t_Array u8 v_PUBLIC_KEY_SIZE = impl_18__as_slice v_PUBLIC_KEY_SIZE self.f_pk
 
 let impl__private_key
       (v_PRIVATE_KEY_SIZE v_PUBLIC_KEY_SIZE: usize)
-      (self: t_KyberKeyPair v_PRIVATE_KEY_SIZE v_PUBLIC_KEY_SIZE)
+      (self: t_MlKemKeyPair v_PRIVATE_KEY_SIZE v_PUBLIC_KEY_SIZE)
     : t_KyberPrivateKey v_PRIVATE_KEY_SIZE = self.f_sk
 
 let impl__public_key
       (v_PRIVATE_KEY_SIZE v_PUBLIC_KEY_SIZE: usize)
-      (self: t_KyberKeyPair v_PRIVATE_KEY_SIZE v_PUBLIC_KEY_SIZE)
+      (self: t_MlKemKeyPair v_PRIVATE_KEY_SIZE v_PUBLIC_KEY_SIZE)
     : t_KyberPublicKey v_PUBLIC_KEY_SIZE = self.f_pk
 
 let impl__sk
       (v_PRIVATE_KEY_SIZE v_PUBLIC_KEY_SIZE: usize)
-      (self: t_KyberKeyPair v_PRIVATE_KEY_SIZE v_PUBLIC_KEY_SIZE)
+      (self: t_MlKemKeyPair v_PRIVATE_KEY_SIZE v_PUBLIC_KEY_SIZE)
     : t_Array u8 v_PRIVATE_KEY_SIZE = impl_12__as_slice v_PRIVATE_KEY_SIZE self.f_sk
