proofs/fstar/extraction/Libcrux.Kem.Kyber.fsti
@@ -35,6 +35,6 @@ val generate_keypair
       (v_K v_CPA_PRIVATE_KEY_SIZE v_PRIVATE_KEY_SIZE v_PUBLIC_KEY_SIZE v_BYTES_PER_RING_ELEMENT v_ETA1 v_ETA1_RANDOMNESS_SIZE:
           usize)
       (randomness: t_Array u8 (sz 64))
-    : Prims.Pure (Libcrux.Kem.Kyber.Types.t_KyberKeyPair v_PRIVATE_KEY_SIZE v_PUBLIC_KEY_SIZE)
+    : Prims.Pure (Libcrux.Kem.Kyber.Types.t_MlKemKeyPair v_PRIVATE_KEY_SIZE v_PUBLIC_KEY_SIZE)
       Prims.l_True
       (fun _ -> Prims.l_True)
